\section{Scaling By Negative One}

\begin{theorem}
  \label{theorem : neg_one_smul}
  \lean{LinearAlgebraGame.neg_one_smul_v}
  \leanok
  \uses{definition : VectorSpace}
  In any vector space $V$ over field $K$, multiplying any vector by $-1$ yields its additive inverse:
  $$\forall v \in V: \quad (-1) \cdot v = -v$$
\end{theorem}

\begin{proof}
  We have $v + (-1) \cdot v = 1 \cdot v + (-1) \cdot v = (1 + (-1)) \cdot v = 0 \cdot v = 0$. Therefore $(-1) \cdot v$ is the additive inverse of $v$, i.e., $(-1) \cdot v = -v$.
\end{proof}